Support separate "forks" #526
This adds _preliminary_ support for forks through the `EvmFork.Fork`
structure.  There remains quite a bit to do, however.  For example,
properly implementing the `LONDON` fork would be an initial goal, along
with updating the tests accordingly.

The essential essence of a fork is twofold: firstly, a sequence of
active EIPs; secondly, a sequence of active bytecodes.  The latter
could, in principle, be derived from the former.  However, to keep
things as simple as possible, for now they are constants.

src/dafny/state.dfy
@@ -16,6 +16,7 @@ include "core/precompiled.dfy"
 include "core/stack.dfy"
 include "core/context.dfy"
 include "core/code.dfy"
+include "core/fork.dfy"
 include "core/storage.dfy"
 include "core/substate.dfy"
 include "core/worldstate.dfy"
@@ -37,6 +38,7 @@ module EvmState {
     import Context
     import SubState
     import Code
+    import opened EvmFork
     import Opcode
     import Precompiled
     import opened Optional
@@ -64,6 +66,7 @@ module EvmState {
      *  @note               Previous remark applies to `gas`.
      */
     datatype Raw = EVM(
+        fork: Fork,
         context: Context.T,
         precompiled: Precompiled.T,
         world : WorldState.T,
@@ -78,7 +81,8 @@ module EvmState {
     // An example instantiation of the EVM to satisfy Dafny's witness
     // requirements.  This should not be consider as a valid or useful instance
     // of the EVM though.
-    const EVM_WITNESS : Raw := EVM(Context.DEFAULT,
+    const EVM_WITNESS : Raw := EVM(BERLIN,
+            Context.DEFAULT,
             Precompiled.DEFAULT,
             WorldState.Create(map[0:=WorldState.DefaultAccount()]),
             EmptyEvmStack,
@@ -153,6 +157,14 @@ module EvmState {
          */
         function IsRevert() : bool {
             this.ERROR? && this.error == REVERTS
+        }
+
+        /**
+         * Get the fork associated with this EVM state.
+         */
+        function Fork() : Fork
+        requires this.EXECUTING? {
+            this.evm.fork
         }
 
         /**
@@ -652,7 +664,7 @@ module EvmState {
      * @param depth The current call depth.
      * @param opcode The opcode causing this call.
      */
-    function Call(world: WorldState.T, ctx: Context.T, precompiled: Precompiled.T, substate: SubState.T, codeAddress: u160, value: u256, gas: nat, depth: nat) : State
+    function Call(world: WorldState.T, ctx: Context.T, fork: Fork, precompiled: Precompiled.T, substate: SubState.T, codeAddress: u160, value: u256, gas: nat, depth: nat) : State
     // Sender account must exist
     requires world.Exists(ctx.sender)  {
         // Address of called contract
@@ -687,7 +699,7 @@ module EvmState {
                         // Construct fresh EVM
                         var stack := EmptyEvmStack;
                         var mem := Memory.Create();
-                        var evm := EVM(ctx,precompiled,nw,stack,mem,cod,substate,gas,0);
+                        var evm := EVM(fork,ctx,precompiled,nw,stack,mem,cod,substate,gas,0);
                         // Off we go!
                         EXECUTING(evm)
     }
@@ -701,7 +713,7 @@ module EvmState {
      * @param gas The available gas to use for the call.
      * @param depth The current call depth.
      */
-    function Create(world: WorldState.T, ctx: Context.T, precompiled: Precompiled.T, substate: SubState.T, initcode: seq<u8>, gas: nat, depth: nat) : State
+    function Create(world: WorldState.T, ctx: Context.T, fork: Fork, precompiled: Precompiled.T, substate: SubState.T, initcode: seq<u8>, gas: nat, depth: nat) : State
     requires |initcode| <= Code.MAX_CODE_SIZE
     requires world.Exists(ctx.sender) {
         var endowment := ctx.callValue;
@@ -726,7 +738,7 @@ module EvmState {
                 var cod := Code.Create(initcode);
                 // Mark new account as having been accessed
                 var ss := substate.AccountAccessed(ctx.address);
-                var evm := EVM(ctx,precompiled,nw,stack,mem,cod,ss,gas,0);
+                var evm := EVM(fork,ctx,precompiled,nw,stack,mem,cod,ss,gas,0);
                 // Off we go!
                 EXECUTING(evm)
     }
@@ -772,7 +784,7 @@ module EvmState {
             // Construct new context
             var ctx := Context.Create(sender,origin,recipient,delegateValue,callData,writePermission,gasPrice,block);
             // Make the call!
-            Call(evm.world,ctx,precompiled,evm.substate,code,callValue,gas,depth+1)
+            Call(evm.world,ctx,evm.fork,precompiled,evm.substate,code,callValue,gas,depth+1)
         }
 
         /**
@@ -825,7 +837,7 @@ module EvmState {
             // Construct new context
             var ctx := Context.Create(sender,origin,address,endowment,[],evm.context.writePermission,gasPrice,block);
             // Make the creation!
-            Create(evm.world,ctx,precompiled,evm.substate,initcode,gas,depth+1)
+            Create(evm.world,ctx,evm.fork,precompiled,evm.substate,initcode,gas,depth+1)
         }
 
         /**
