src/test/dafny/proofs/Push.dfy
@@ -1,5 +1,4 @@
 include "../../../dafny/evm.dfy"
-include "../../../dafny/evms/berlin.dfy"
 
 import opened EvmState
 import opened Code
